ring-buffer: finish simulation proofs

examples/ring/CellASpec.v
@@ -50,6 +50,44 @@ Module CellAS. Section CellAS.
     Seal.sealing "CellAS"
       (OwnM (auth_r v)).
 
+  Lemma pending_unique : pending -∗ pending -∗ False.
+  Proof.
+    rewrite /pending /pending_r; unseal "CellAS".
+    iIntros "P P'"; iCombine "P P'" as "P" gives %FALSE; rewrite -pair_op pair_valid in FALSE; des; ss.
+    rr in FALSE; specialize (FALSE idx); des_ifs.
+  Qed.
+
+  Lemma cell_unique v v':
+    cell v -∗ cell v' -∗ False.
+  Proof.
+    rewrite /cell /auth /cell_r /cellraw_r; unseal "CellAS".
+    iIntros "P P'"; iCombine "P P'" as "P" gives %FALSE; rewrite -pair_op pair_valid in FALSE; des; ss.
+    rewrite -auth_frag_op in FALSE0; apply auth_frag_valid_1 in FALSE0.
+    rr in FALSE0; specialize (FALSE0 idx); des_ifs.
+  Qed.
+
+  Lemma cell_auth_get v v':
+    cell v' -∗ auth v -∗ ⌜v = v'⌝.
+  Proof.
+    rewrite /cell /auth /cell_r; unseal "CellAS"; rewrite /auth_r /cellraw_r.
+    iIntros "P P'"; iCombine "P P'" as "P" gives %wf.
+    rewrite -pair_op pair_valid auth_both_valid_discrete /= in wf; des.
+    apply (discrete_fun_included_spec_1 _ _ idx) in wf0; ss;
+    des_ifs.
+    by rewrite Excl_included in wf0.
+  Qed.
+
+  Lemma cell_auth_set v v':
+    cell v -∗ auth v -∗ |==> cell v' ∗ auth v'.
+  Proof.
+    rewrite /cell /auth /cell_r; unseal "CellAS"; rewrite /auth_r /cellraw_r.
+    iIntros "C AU". iCombine "C AU" as "H".
+    iMod (OwnM_Upd with "H") as "[C AU]"; last by (iModIntro; iSplitL "AU"). 
+    rewrite comm; apply prod_update, auth_update, discrete_fun_local_update; intros x; ss.
+    destruct (decide (idx = x)); subst; des_ifs.
+    apply option_local_update, exclusive_local_update; ss.
+  Qed.
+
   Definition get_spec : fspec :=
     fspec_simple (fun v: Z =>
      ((fun arg => ⌜arg = tt↑⌝ ∗ cell v),
@@ -61,12 +99,12 @@ Module CellAS. Section CellAS.
       (fun ret => ⌜ret = tt↑⌝ ∗ cell v)))%I.
 
   Definition Stb : alist gname fspec :=
-    Seal.sealing "CellAS" [(CellName.get idx, get_spec);
+    Seal.sealing "ccr" [(CellName.get idx, get_spec);
                         (CellName.set idx, set_spec)].
 
   Lemma Stb_nodup : List.NoDup (List.map fst Stb).
   Proof.
-    unfold Stb. unseal "CellAS". prove_nodup.
+    unfold Stb. unseal "ccr". prove_nodup.
   Qed.
   
 End CellAS. End CellAS.
