examples/ring/CellIAproof.v
@@ -1,105 +1,46 @@
-(*
-Require Import Coqlib ITreelib sflib.
+Require Import Coqlib ITreelib.
 Require Import ImpPrelude.
 Require Import Skeleton.
-Require Import IPM.
+Require Import IPM sWorld.
 Require Import Events Behavior.
 Require Import Relation_Definitions.
 
-(*** TODO : export these in Coqlib or Universe ***)
-Require Import Relation_Operators.
-Require Import RelationPairs.
-From ITree Require Import
-     Events.MapDefault.
-From ExtLib Require Import
-     Core.RelDec
-     Structures.Maps
-     Data.Map.FMapAList.
-Require Import STB.
-Require Import IPM STB sProp sWorld.
+Require Import CellHeader CellASpec CellI SMod ModSim.
+Require Import CellA STB.
 
-Require Import ISim ITactics SMod HMod PMod Events.
-Require Import Mod ModSim ModSimFacts.
-Require Import sProp sWorld.
-Require Import CellHeader CellASpec CellA CellI.
+Require Import ISim HMod PMod Events ITactics.
+Require Import Mod ModSimFacts.
 
 Set Implicit Arguments.
 
 Local Open Scope nat_scope.
 
-Module CellIA.
-Section SIMMODSEM.
+(* Simulation Proof *)
+Module CellIA. Section CellIA.
+  Import CellAS.
   Context `{!Inv.t Σ Γ α β τ, !CellAS.G Γ}.
   Notation iProp := (iProp Σ).
 
   Variable idx : nat.
 
-  Variable GI : Sk.t -> invspec.
-  Variable StbG : Sk.t -> gname -> option fspec.
-
-  Import CellAS.
-
-  Lemma pending_unique : pending idx -∗ pending idx -∗ False.
-  Proof.
-    rewrite /pending /pending_r; unseal "CellAS".
-    iIntros "P P'"; iCombine "P P'" as "P" gives %FALSE; rewrite -pair_op pair_valid in FALSE; des; ss.
-    rr in FALSE; specialize (FALSE idx); des_ifs.
-  Qed.
-
-  Lemma cell_unique v v':
-    cell idx v -∗ cell idx v' -∗ False.
-  Proof.
-    rewrite /cell /auth /cell_r /cellraw_r; unseal "CellAS".
-    iIntros "P P'"; iCombine "P P'" as "P" gives %FALSE; rewrite -pair_op pair_valid in FALSE; des; ss.
-    rr in FALSE0; specialize ()
-    .
-  Qed.
-
-  Lemma cell_auth_get v v':
-    cell idx v' -∗ auth idx v -∗ ⌜v = v'⌝.
-  Proof.
-    unfold cell, auth. unseal "ccr". unfold cell_r, auth_r, cellraw_r.
-    iIntros "H0 H1". iCombine "H0 H1" as "H".
-    iOwnWf "H" as WF. iPureIntro. rr in WF. ur in WF. unseal "ra". des.
-    rr in WF0. ur in WF0. unseal "ra". des.
-    rr in WF0. des. ur in WF0. eapply equal_f with (x:=idx) in WF0.
-    ur in WF0. des_ifs.
-  Qed.
-
-  Lemma cell_auth_set v v':
-    cell idx v -∗ auth idx v -∗ |==> cell idx v' ∗ auth idx v'.
-  Proof.
-    unfold cell, auth. unseal "ccr".
-    iIntros "H0 H1". iCombine "H0 H1" as "H".
-    iPoseProof (OwnM_Upd with "H") as "H".
-    { instantiate (1:= (cell_r idx v') ⋅ (auth_r idx v')).
-      unfold cell_r, auth_r, cellraw_r.
-      rr. intros ctx WF. ur in WF. ur. unseal "ra". des_ifs. des. split; auto.
-      ur in WF0. ur. des_ifs. des. rr in WF0. des. split.
-      { rr. exists ctx. ur in WF0. ur. extensionality n.
-        eapply equal_f with (x:=n) in WF0. ur in WF0. ur.
-        des_ifs; rewrite ->?fn_lookup_insert, ?fn_lookup_insert_ne; eauto.
-      }
-      { ur. i. rr. ur. unseal "ra". des_ifs. }
-    }
-    iMod "H". iDestruct "H" as "[H0 H1]". iFrame. auto.
-  Qed.
-
   Definition Ist : Sk.t -> nat -> alist key Any.t -> alist key Any.t -> iProp :=
-    (fun _ _ st_src st_tgt =>
-       ∃vany v, ⌜st_tgt = [(CellI.v_cv idx, vany)]⌝ ∗
-       ((cell idx v ∗ auth idx v)
-        ∨
-        (⌜vany = v↑⌝ ∗ pending idx ∗ auth idx v)))%I.
+    (λ _ _ st_src st_tgt,
+       ∃ vany v, 
+        ⌜st_tgt = [(CellI.v_cv idx, vany)]⌝
+        ∗ ((cell idx v ∗ auth idx v)
+          ∨ (⌜vany = v↑⌝ ∗ pending idx ∗ auth idx v)))%I.
 
+  Variable ginv : Sk.t -> invspec.
+  Variable StbCell : Sk.t -> gname -> option fspec.
+
+  Local Notation CellA := (CellA.t idx ginv StbCell).
   Local Notation CellI := (CellI.t idx).
-  Local Notation CellA := (CellA.t idx GI StbG).
 
-  Lemma simF_get:
-    HSim.sim_fun CellA CellI Ist (CellName.get idx).
+  Lemma simF_get : HSim.sim_fun CellA CellI Ist (CellName.get idx).
   Proof.
     init_simF.
 
+    (* SRC: handle the IST of the Cell and the precond of get *)
     steps_l. iDestruct "ASM" as "((% & C) & %)". subst. hss.
     iDestruct "IST" as (vany v0) "(% & [(C' & A)|(% & P & A)])".
     { iExFalso. iApply (cell_unique with "C' C"). }
@@ -162,5 +103,4 @@ Section SIMMODSEM.
     - apply simF_set.
   Qed.
 
-End SIMMODSEM.
-End CellIA. *)
+End CellIA. End CellIA.
