examples/ring/RingASpec.v
@@ -17,14 +17,14 @@ Module RingAS. Section RingAS.
   Context `{Σ : GRA.t}.
 
   Definition Stb : alist gname fspec :=
-    Seal.sealing "RingAS" [(RingName.init, fspec_trivial);
+    Seal.sealing "ccr" [(RingName.init, fspec_trivial);
                           (RingName.get_size, fspec_trivial);
                           (RingName.enqueue, fspec_trivial);
                           (RingName.dequeue, fspec_trivial)].
 
   Lemma Stb_nodup : List.NoDup (List.map fst Stb).
   Proof.
-    unfold Stb. unseal "RingAS". prove_nodup.
+    unfold Stb. unseal "ccr". prove_nodup.
   Qed.
   
 End RingAS.
