examples/ring/CellI.v
@@ -49,6 +49,6 @@ Module CellI. Section CellI.
   |}
   .
 
-  Definition t := Seal.sealing "CRIS" (PMod.to_hmod Mod).
+  Definition t := Seal.sealing "ccr" (PMod.to_hmod Mod).
 
 End CellI. End CellI.
